theories/aneris_lang/lib/nodup.v
@@ -5,16 +5,16 @@ Set Default Proof Using "Type".
 Import Network.
 
 Definition receivefrom_nodup : val :=
-  λ: "socket" "msgs",
+  λ: "rcvlog" "socket",
   (rec: "loop" <> :=
      let: "msg" := unSOME (ReceiveFrom "socket") in
-     if: set_mem "msg" "msgs" then "loop" #()
-     else ("msg", set_add "msg" "msgs")) #().
+     if: set_mem "msg" "rcvlog" then "loop" #()
+     else ("msg", set_add "msg" "rcvlog")) #().
 
 Definition receivefrom_nodup_n : val :=
   rec: "receivefrom_nodup_n" "socket" "msgs" "n" :=
     if: "n" = #0 then (list_nil, "msgs") else
-    let: "tmp" := receivefrom_nodup "socket" "msgs" in
+    let: "tmp" := receivefrom_nodup "msgs" "socket" in
     let: "m" := Fst "tmp" in
     let: "msgs'" := Snd "tmp" in
     let: "tailmsgs" := "receivefrom_nodup_n" "socket" "msgs'" ("n" - #1) in
@@ -22,25 +22,49 @@ Definition receivefrom_nodup_n : val :=
     let: "msgs''" := Snd "tailmsgs" in
     ("m" :: "ms", "msgs''").
 
-Definition nodup_init : val := set_empty.
+Definition nodup_empty : val := set_empty.
+
+Definition nodup_init : val :=
+  λ: <>,
+    let: "log" := ref (nodup_empty #()) in
+    λ: "socket",
+      let: "tmp"  := receivefrom_nodup !"log" "socket" in
+      let: "msg"  := Fst "tmp" in
+      let: "log'" := Snd "tmp" in
+      "log" <- "log'";;
+      "msg".
+
+Definition receivefrom_nodup_set : val :=
+  λ: "socket" "rcv" "addrs",
+  let: "sndrs" := ref (set_empty #()) in
+  let: "msgs"  := ref (set_empty #()) in
+  (rec: "loop" <> :=
+     if: set_equal !"sndrs" "addrs" then !"msgs" else
+     let: "msg" := "rcv" "socket" in
+     let: "sndr" := Snd "msg" in
+     (* if: set_mem "sndr" !"sndrs" then "loop" #() *)
+     (* else *)
+     "sndrs" <- set_add "sndr" !"sndrs";;
+     "msgs"  <- set_add "msg"  !"msgs";;
+     "loop" #()) #().
 
 Section nodup_specs.
   Context `{dG : anerisG Mdl Σ}.
 
-  Local Definition msg_toval : message_body * socket_address → val :=
+  Definition msg_toval : message_body * socket_address → val :=
     λ '(b, s), (#b, #s)%V.
 
   Local Instance: Inj (=) (=) msg_toval.
   Proof. intros [] []. by inversion 1; simplify_eq. Qed.
 
-  Definition is_nodup (R : gset message) (a : socket_address) (v : val) : Prop :=
+  Definition is_rcvset (R : gset message) (a : socket_address) (v : val) : Prop :=
     is_set msg_toval (gset_map (λ m, (m_body m, m_sender m)) R) v ∧
     set_Forall (λ m, m_destination m = a) R.
 
-  Lemma wp_nodup_init a :
+  Lemma wp_nodup_empty a :
     {{{ True }}}
-      nodup_init #() @[ip_of_address a]
-    {{{ v, RET v; ⌜is_nodup (∅ : gset message) a v⌝ }}}.
+      nodup_empty #() @[ip_of_address a]
+    {{{ v, RET v; ⌜is_rcvset (∅ : gset message) a v⌝ }}}.
   Proof.
     iIntros (Φ) "_ HΦ".
     wp_apply (wp_set_empty msg_toval); [done|].
@@ -52,11 +76,11 @@ Section nodup_specs.
     ip = ip_of_address a →
     saddress s = Some a →
     sblock s = true →
-    {{{ h ↪[ip] s ∗ a ⤇ φ ∗ a ⤳ (R, T) ∗ ⌜is_nodup R a v⌝ }}}
-      receivefrom_nodup #(LitSocket h) v @[ip]
+    {{{ h ↪[ip] s ∗ a ⤇ φ ∗ a ⤳ (R, T) ∗ ⌜is_rcvset R a v⌝ }}}
+      receivefrom_nodup v #(LitSocket h) @[ip]
     {{{ m v', RET ((#(m_body m), #(m_sender m)), v')%V;
           h ↪[ip] s ∗ a ⤳ ({[m]} ∪ R, T) ∗ φ m ∗
-          ⌜is_nodup ({[m]} ∪ R) a v'⌝ ∗ ⌜m ∉ R⌝ }}}.
+          ⌜is_rcvset ({[m]} ∪ R) a v'⌝ ∗ ⌜m ∉ R⌝ }}}.
   Proof.
     iIntros (-> ?? Φ) "(Hh & #Hφ & Ha & [%Hv %Hdest]) HΦ".
     wp_rec. do 3 wp_pure _.
@@ -95,10 +119,10 @@ Section nodup_specs.
     ip = ip_of_address a →
     saddress s = Some a →
     sblock s = true →
-    {{{ h ↪[ip] s ∗ a ⤇ φ ∗ a ⤳ (R, T) ∗ ⌜is_nodup R a v⌝ }}}
+    {{{ h ↪[ip] s ∗ a ⤇ φ ∗ a ⤳ (R, T) ∗ ⌜is_rcvset R a v⌝ }}}
       receivefrom_nodup_n #(LitSocket h) v #n @[ip]
     {{{ ms vms v' R', RET (vms, v')%V;
-          ⌜is_nodup R' a v'⌝ ∗ ⌜length ms = n⌝ ∗
+          ⌜is_rcvset R' a v'⌝ ∗ ⌜length ms = n⌝ ∗
           ⌜is_list (map (λ m, (#(m_body m), #(m_sender m))%V) ms) vms⌝ ∗
           h ↪[ip] s ∗ a ⤳ (R', T) ∗ [∗ list] m ∈ ms, φ m }}}.
   Proof.
@@ -117,6 +141,114 @@ Section nodup_specs.
     iApply ("HΦ" $! (m :: ms)).
     iFrame. iFrame "%".
     simpl. rewrite Hlen //.
+  Qed.
+
+  Definition is_rcvset_log l R a : iProp Σ :=
+    ∃ log, l ↦[ip_of_address a] log ∗ ⌜is_rcvset R a log⌝.
+
+  Definition wp_nodup_rcv (rcv : val) a s l : iProp Σ :=
+    □ (∀ h φ R T,
+          {{{ h ↪[ip_of_address a] s ∗ a ⤇ φ ∗ a ⤳ (R, T) ∗ is_rcvset_log l R a }}}
+            rcv #(LitSocket h) @[ip_of_address a]
+          {{{ m, RET (#(m_body m), #(m_sender m))%V;
+                h ↪[ip_of_address a] s ∗ a ⤳ ({[m]} ∪ R, T) ∗ φ m ∗
+                is_rcvset_log l ({[m]} ∪ R) a ∗ ⌜m ∉ R⌝ }}}).
+
+  Lemma wp_nodup_init a s :
+    saddress s = Some a →
+    sblock s = true →
+    {{{ True }}}
+      nodup_init #() @[ip_of_address a]
+    {{{ l rcv, RET rcv; is_rcvset_log l ∅ a ∗ wp_nodup_rcv rcv a s l }}}.
+  Proof.
+    iIntros (?? Φ) "_ HΦ".
+    rewrite /nodup_init. wp_pures.
+    wp_apply wp_nodup_empty; [done|].
+    iIntros (log Hlog).
+    wp_alloc l as "Hl". wp_pures.
+    iApply "HΦ".
+    iSplitL "Hl".
+    { iExists _. by iFrame. }
+    iIntros "!#" (h φ R T Ψ) "!# (Hh & #Hφ & Ha & Hrcv) HΨ".
+    iDestruct "Hrcv" as (log') "[Hl %HR]".
+    wp_pures. wp_load.
+    wp_apply (wp_receivefrom_nodup with "[$Hh $Ha $Hφ //]"); [done..|].
+    iIntros (m v) "(Hh & Ha & Hm & % & %)".
+    wp_pures. wp_store.
+    iApply "HΨ". iFrame. iFrame "%".
+    iExists _. by iFrame.
+  Qed.
+
+  Global Instance :  Inj (=) (=) (LitV ∘ LitSocketAddress).
+  Proof. intros ??. by inversion 1. Qed.
+
+  Lemma wp_receivefrom_set ip a φ h s R T addrs av (rcv : val) l :
+    ip = ip_of_address a →
+    saddress s = Some a →
+    sblock s = true →
+    □ (∀ m, φ m → ⌜m_sender m ∈ addrs⌝)%I -∗
+    wp_nodup_rcv rcv a s l -∗
+    {{{ h ↪[ip] s ∗ a ⤇ φ ∗ a ⤳ (R, T) ∗ is_rcvset_log l R a ∗
+        ⌜is_set (LitV ∘ LitSocketAddress) addrs av⌝ }}}
+      receivefrom_nodup_set #(LitSocket h) rcv av @[ip]
+    {{{ ms mv R', RET mv;
+          ⌜is_set msg_toval (gset_map (λ m, (m_body m, m_sender m)) ms) mv⌝ ∗
+          h ↪[ip] s ∗ a ⤳ (R', T) ∗ is_rcvset_log l R' a ∗
+          ([∗ set] n ∈ addrs, ∃ m, ⌜m ∈ ms⌝ ∗ ⌜m_sender m = n⌝ ∗ φ m) }}}.
+  Proof.
+    iIntros (-> ??) "#Hincl #Hrecv". iIntros (Φ) "!# (Hh & #Hφ & Ha & Hlog & %Haddrs) HΦ".
+    rewrite /receivefrom_nodup_set. wp_pures.
+    wp_apply (wp_set_empty (LitV ∘ LitSocketAddress)); [done|].
+    iIntros (vsndrs Hsndrs).
+    wp_alloc lsndr as "Hsndr". wp_pures.
+    wp_apply (wp_set_empty msg_toval); [done|].
+    iIntros (vmsgs Hmsg).
+    wp_alloc lmsg as "Hmsg". do 3 wp_pure _.
+    iAssert (∃ sndrs msgs vsndrs vmsgs,
+                lsndr ↦[ip_of_address a] vsndrs ∗
+                lmsg  ↦[ip_of_address a] vmsgs ∗
+                ⌜is_set (LitV ∘ LitSocketAddress) sndrs vsndrs⌝ ∗
+                ⌜is_set msg_toval (gset_map (λ m, (m_body m, m_sender m)) msgs) vmsgs⌝ ∗
+                [∗ set] n ∈ sndrs, ∃ m, ⌜m ∈ msgs⌝ ∗ ⌜m_sender m = n⌝ ∗ φ m)%I
+      with "[Hmsg Hsndr]" as "Hlogs".
+    { iExists ∅, ∅, _, _. iFrame. by iFrame "%". }
+    clear Hsndrs vsndrs Hmsg vmsgs.
+    iLöb as "IH" forall (R).
+    wp_pures.
+    iDestruct "Hlogs" as (sndrs msgs vsendrs vmsgs)
+                           "(Hsndrs & Hmsgs & % & % & Hms)".
+    wp_load.
+    wp_apply (wp_set_equal (LitV ∘ LitSocketAddress)); [auto|].
+    iIntros ([] Hb); wp_if.
+    { wp_load. iApply ("HΦ" $! msgs). rewrite Hb. by iFrame. }
+    wp_apply ("Hrecv" with "[$Hh $Hφ $Ha $Hlog]").
+    iIntros (m) "(Hh & Ha & Hm & Hlog & %)".
+    wp_pures. wp_load.
+    wp_apply (wp_set_add (LitV ∘ LitSocketAddress) with "[//]").
+    iIntros (vsndrs' Hsndrs'). wp_store.
+    wp_load.
+    wp_apply (wp_set_add msg_toval _ (_,_)  with "[//]").
+    iIntros (vmsgs' Hmsgs').
+    wp_store.
+    iApply ("IH" with "Hh Ha Hlog [HΦ]"); last first.
+    { iExists ({[m_sender m]} ∪ sndrs), ({[m]} ∪ msgs), _, _.
+      iFrame.
+      rewrite -(gset_map_singleton (λ m, (m_body m, m_sender m)) m)
+              -gset_map_union in Hmsgs'.
+      iFrame "%".
+      destruct (decide (m_sender m ∈ sndrs)).
+      { assert ({[m_sender m]} ∪ sndrs = sndrs) as -> by set_solver.
+        iApply (big_sepS_impl with "Hms").
+        iIntros "!#" (??). iDestruct 1 as (m') "(% & % & ?)".
+        iExists m'. iFrame. iFrame "%". iPureIntro; set_solver. }
+      rewrite big_sepS_union ?big_sepS_singleton; [|set_solver].
+      iSplitL "Hm".
+      { iExists m. iFrame. iSplit; [|done]. iPureIntro; set_solver. }
+      iApply (big_sepS_impl with "Hms").
+      iIntros "!#" (??). iDestruct 1 as (m') "(% & % & ?)".
+      iExists m'. iFrame. iFrame "%". iPureIntro; set_solver. }
+    iIntros (???) "(% & Hh & Ha & Hl & Hms)".
+    iApply "HΦ". by iFrame.
   Qed.
 
 End nodup_specs.
