theories/aneris_lang/lib/set.v
@@ -1,10 +1,27 @@
 From aneris.aneris_lang Require Import proofmode.
 From aneris.aneris_lang.lib Require Import list.
+From iris_string_ident Require Import ltac2_string_ident.
 Set Default Proof Using "Type".
 
 Definition set_empty : val := λ: <>, [].
-Definition set_add : val := list_cons.
+
+Definition set_add : val :=
+  λ: "x" "X",
+  if: list_mem "x" "X" then "X"
+  else "x" :: "X".
+
 Definition set_mem : val := list_mem.
+
+Definition set_iter : val := list_iter.
+
+Definition set_forall : val := list_forall.
+
+Definition set_subseteq : val :=
+  λ: "X" "Y",
+  list_forall (λ: "x", set_mem "x" "Y") "X".
+
+Definition set_equal : val :=
+  λ: "X" "Y", set_subseteq "X" "Y" && set_subseteq "Y" "X".
 
 Section set_specs.
   Context `{anerisG Mdl Σ}.
@@ -12,7 +29,7 @@ Section set_specs.
   Context (toval : A → val).
 
   Definition is_set (X : gset A) (v : val) : Prop :=
-    ∃ (l : list A), is_list (map toval l) v ∧ X = list_to_set l.
+    ∃ (l : list A), is_list (map toval l) v ∧ X = list_to_set l ∧ NoDup l.
 
   Lemma wp_set_empty  ip :
     {{{ True }}}
@@ -22,18 +39,27 @@ Section set_specs.
     iIntros (Φ) "_ HΦ".
     wp_rec. wp_pures. iApply "HΦ".
     iExists []. repeat iSplit; auto.
+    iPureIntro; by apply NoDup_nil.
   Qed.
 
-  Lemma wp_set_add ip x X v :
+  Lemma wp_set_add `{!Inj (=) (=) toval} ip x X v :
     {{{ ⌜is_set X v⌝ }}}
       set_add (Val (toval x)) (Val v) @[ip]
     {{{ v, RET v; ⌜is_set ({[ x ]} ∪ X) v⌝}}}.
   Proof.
-    iIntros (Φ (? & ? & ->)) "HΦ".
-    wp_apply (wp_list_cons with "[//]").
-    iIntros (v' Hv').
-    iApply "HΦ".
-    iExists (_ :: _); eauto.
+    iIntros (Φ (l & ? & -> & Hdup)) "HΦ".
+    wp_rec; wp_pures.
+    wp_apply (wp_list_mem _ l with "[//]"); [done|].
+    iIntros ([] Hb); wp_if.
+    - iApply "HΦ". iPureIntro.
+      exists l. do 2 (split; auto).
+      set_solver.
+    - wp_apply (wp_list_cons with "[//]").
+      iIntros (v' Hv').
+      iApply "HΦ". iPureIntro.
+      eexists (_ :: _).
+      repeat split; auto.
+      destruct Hb; subst; constructor; auto with set_solver.
   Qed.
 
   Lemma wp_set_mem `{!Inj (=) (=) toval} ip x X v :
@@ -41,11 +67,82 @@ Section set_specs.
       set_mem (Val (toval x)) (Val v) @[ip]
    {{{ (b : bool), RET #b; ⌜if b then x ∈ X else x ∉ X⌝ }}}.
   Proof.
-    iIntros (Φ (l & ? & ->)) "HΦ".
+    iIntros (Φ (l & ? & -> & ?)) "HΦ".
     iApply (wp_list_mem _ l with "[//]"); [done|].
     iIntros ([] Hb); iApply "HΦ"; iPureIntro.
     { set_solver. }
     destruct Hb; set_solver.
+  Qed.
+
+  Lemma wp_set_iter Φ Ψ P ip (X : gset A) v handler :
+    (∀ (x : A),
+       {{{ ⌜x ∈ X⌝ ∗ P ∗ Φ x }}}
+         (Val handler) (toval x) @[ip]
+       {{{v, RET v; P ∗ Ψ x }}}) -∗
+    {{{ ⌜is_set X v⌝ ∗ P ∗ [∗ set] x ∈ X, Φ x }}}
+      set_iter (Val handler) (Val v) @[ip]
+    {{{ RET #(); P ∗ [∗ set] x ∈ X, Ψ x }}}.
+  Proof.
+    iIntros "#Hhandler".
+    iIntros "!#" (Ξ) "(%HX & HP & HΦ) HΞ".
+    destruct HX as (l & ? & -> & Hdup).
+    rewrite !big_sepS_list_to_set //.
+    wp_apply (wp_list_iter Φ Ψ P with "[] [$HP $HΦ //]"); [|done].
+    iIntros (a) "!#". iIntros (Ξ') "(%Ha & HP & HΦ) HΞ' ".
+    wp_apply ("Hhandler" with "[$HP $HΦ]"); [|done].
+    iPureIntro; set_solver.
+  Qed.
+
+  Lemma wp_set_subseteq `{!Inj (=) (=) toval} ip X Y xv yv:
+    {{{ ⌜is_set X xv⌝ ∗ ⌜is_set Y yv⌝}}}
+      set_subseteq (Val xv) (Val yv) @[ip]
+    {{{ (b : bool), RET #b; ⌜if b then X ⊆ Y else X ⊈ Y⌝ }}}.
+  Proof.
+    iIntros (Φ) "[%HX %HY] HΦ".
+    destruct HX as (Xl & ? & -> & ?).
+    rewrite /set_subseteq. wp_pures.
+    wp_apply (wp_list_forall (λ x, ⌜x ∈ Y⌝) (λ x, ⌜x ∉ Y⌝) with "[] [//]")%I.
+    { iIntros (x v Ψ) "!#". iIntros (->) "HΨ".
+      wp_pures. wp_apply (wp_set_mem with "[//]").
+      iIntros ([] ?); by iApply "HΨ". }
+    iIntros ([]) "Hb".
+    - iApply "HΦ".
+      rewrite elem_of_subseteq.
+      iIntros (x Hx%elem_of_list_to_set).
+      rewrite big_sepL_elem_of //.
+    - iApply "HΦ". iDestruct "Hb" as (x) "[% %]".
+      iPureIntro; set_solver.
+  Qed.
+
+  Lemma wp_set_equal `{!Inj (=) (=) toval} ip X Y xv yv:
+    {{{ ⌜is_set X xv⌝ ∗ ⌜is_set Y yv⌝}}}
+      set_equal (Val xv) (Val yv) @[ip]
+    {{{ (b : bool), RET #b; ⌜if b then X = Y else X ≠ Y⌝ }}}.
+  Proof.
+    iIntros (Φ) "[%HX %HY] HΦ".
+    rewrite /set_equal. wp_pures.
+    wp_apply (wp_set_subseteq); [auto|].
+    iIntros ([] ?); wp_if; last first.
+    { iApply "HΦ". iPureIntro; set_solver. }
+    wp_apply (wp_set_subseteq); [auto|].
+    iIntros ([] ?); iApply "HΦ"; iPureIntro; set_solver.
+  Qed.
+
+  Lemma wp_set_forall Φ Ψ ip X xv (fv : val) :
+    (∀ (a : A) av,
+        {{{ ⌜av = toval a⌝ }}}
+          fv av @[ip]
+        {{{ (b : bool), RET #b; if b then Φ a else Ψ a }}}) -∗
+    {{{ ⌜is_set X xv⌝ }}}
+      list_forall fv xv @[ip]
+    {{{ (b : bool), RET #b; if b then [∗ set] x ∈ X, Φ x else ∃ x, ⌜x ∈ X⌝ ∗ Ψ x }}}.
+  Proof.
+    iIntros "#Hfv !#" (Ξ (?&?&->&?)) "HΞ".
+    wp_apply (wp_list_forall with "[//] [//]").
+    iIntros ([]) "Hb"; iApply "HΞ".
+    { rewrite  big_sepS_list_to_set //. }
+    iDestruct "Hb" as (?) "[% ?]".
+    iExists _. rewrite elem_of_list_to_set. eauto.
   Qed.
 
 End set_specs.
